theories/typing.v
@@ -8,7 +8,7 @@ Require Import RecordUpdate.RecordUpdate.
 Require Import RichWasm.syntax.
 
 Record module_ctx :=
-  { mc_globals : list global_type }.
+  { mc_globals : list (mutability * type) }.
 
 Definition local_ctx := list type.
 
@@ -18,7 +18,6 @@ Record function_ctx :=
     fc_location_vars : nat;
     fc_own_vars : nat;
     fc_rep_vars : nat;
-    fc_sizity_vars : nat;
     fc_size_vars : nat;
     fc_type_vars : list kind }.
 
@@ -28,42 +27,41 @@ Definition fc_empty : function_ctx :=
      fc_location_vars := 0;
      fc_own_vars := 0;
      fc_rep_vars := 0;
-     fc_sizity_vars := 0;
      fc_size_vars := 0;
      fc_type_vars := [] |}.
 
 Global Instance eta_function_ctx : Settable _ :=
   settable! Build_function_ctx
-  <fc_result_type; fc_labels; fc_location_vars; fc_own_vars; fc_rep_vars; fc_sizity_vars;
-   fc_size_vars; fc_type_vars>.
+  <fc_result_type; fc_labels; fc_location_vars; fc_own_vars; fc_rep_vars; fc_size_vars;
+   fc_type_vars>.
 
 Definition update_locals (le : local_effect) (L : local_ctx) : local_ctx :=
   fold_left (fun acc '(i, τ) => <[ i := τ ]> acc) le L.
 
 Inductive rep_ok : function_ctx -> representation -> Prop :=
-| VarR_OK (F : function_ctx) (ϱ : variable) :
-  ϱ < F.(fc_rep_vars) -> rep_ok F (VarR ϱ)
-| SumR_OK (F : function_ctx) (rs : list representation) :
-  Forall (rep_ok F) rs -> rep_ok F (SumR rs)
-| ProdR_OK (F : function_ctx) (rs : list representation) :
-  Forall (rep_ok F) rs -> rep_ok F (ProdR rs)
-| PrimR_OK (F : function_ctx) (p : primitive_rep) :
-  rep_ok F (PrimR p).
+| VarR_OK (F : function_ctx) (r : variable) :
+  r < F.(fc_rep_vars) -> rep_ok F (VarR r)
+| SumR_OK (F : function_ctx) (ρs : list representation) :
+  Forall (rep_ok F) ρs -> rep_ok F (SumR ρs)
+| ProdR_OK (F : function_ctx) (ρs : list representation) :
+  Forall (rep_ok F) ρs -> rep_ok F (ProdR ρs)
+| PrimR_OK (F : function_ctx) (ι : primitive_rep) :
+  rep_ok F (PrimR ι).
 
 Inductive kind_ok : function_ctx -> kind -> Prop :=
-| VALTYPE_OK (F : function_ctx) (r : representation) (l : linearity) (h : heapability) :
-  rep_ok F r -> kind_ok F (VALTYPE r h l)
-| MEMTYPE_OK (F : function_ctx) (sy : sizity) :
-  kind_ok F (MEMTYPE sy).
+| VALTYPE_OK (F : function_ctx) (ρ : representation) (η : heapability) (γ : linearity) :
+  rep_ok F ρ -> kind_ok F (VALTYPE ρ η γ)
+| MEMTYPE_OK (F : function_ctx) (ζ : sizity) :
+  kind_ok F (MEMTYPE ζ).
 
 Inductive mono_rep : representation -> list primitive_rep -> Prop :=
-| MonoSumR (rs : list representation) (pss : list (list primitive_rep)) :
-  Forall2 mono_rep rs pss ->
+| MonoSumR (ρs : list representation) (ιss : list (list primitive_rep)) :
+  Forall2 mono_rep ρs ιss ->
   (* TODO: Use an efficient packing. *)
-  mono_rep (SumR rs) (concat pss)
-| MonoProdR (rs : list representation) (pss : list (list primitive_rep)) :
-  Forall2 mono_rep rs pss ->
-  mono_rep (ProdR rs) (concat pss)
+  mono_rep (SumR ρs) (concat ιss)
+| MonoProdR (ρs : list representation) (ιss : list (list primitive_rep)) :
+  Forall2 mono_rep ρs ιss ->
+  mono_rep (ProdR ρs) (concat ιss)
 | MonoPtrR :
   mono_rep (PrimR PtrR) [PtrR]
 | MonoI32R :
@@ -75,8 +73,8 @@ Inductive mono_rep : representation -> list primitive_rep -> Prop :=
 | MonoF64R :
   mono_rep (PrimR F64R) [F64R].
 
-Definition primitive_size (p : primitive_rep) : nat :=
-  match p with
+Definition primitive_size (ι : primitive_rep) : nat :=
+  match ι with
   | PtrR => 1
   | I32R => 1
   | I64R => 2
@@ -85,21 +83,24 @@ Definition primitive_size (p : primitive_rep) : nat :=
   end.
 
 Inductive has_mono_size : representation -> nat -> Prop :=
-| MonoSize (r : representation) (ps : list primitive_rep) :
-  mono_rep r ps ->
-  has_mono_size r (list_sum (map primitive_size ps)).
+| MonoSize (ρ : representation) (ιs : list primitive_rep) :
+  mono_rep ρ ιs ->
+  has_mono_size ρ (list_sum (map primitive_size ιs)).
 
 Inductive has_kind : function_ctx -> type -> kind -> Prop :=
-| KSubLin F τ r h :
-  has_kind F τ (VALTYPE r h Unr) ->
-  has_kind F τ (VALTYPE r h Lin)
-| KSubHeap F τ r l :
-  has_kind F τ (VALTYPE r Heapable l) ->
-  has_kind F τ (VALTYPE r Unheapable l)
-| KVar F α κ :
-  F.(fc_type_vars) !! α = Some κ ->
+| KSubLin F τ ρ η :
+  has_kind F τ (VALTYPE ρ η Unr) ->
+  has_kind F τ (VALTYPE ρ η Lin)
+| KSubUnheapable F τ ρ γ :
+  has_kind F τ (VALTYPE ρ Heapable γ) ->
+  has_kind F τ (VALTYPE ρ Unheapable γ)
+| KSubUnsized F τ σ :
+  has_kind F τ (MEMTYPE (Sized σ)) ->
+  has_kind F τ (MEMTYPE Unsized)
+| KVar F t κ :
+  F.(fc_type_vars) !! t = Some κ ->
   kind_ok F κ ->
-  has_kind F (VarT α) κ
+  has_kind F (VarT t) κ
 | KI32 F :
   has_kind F (NumT (IntT I32T)) (VALTYPE (PrimR I32R) Heapable Unr)
 | KI64 F :
@@ -108,24 +109,27 @@ Inductive has_kind : function_ctx -> type -> kind -> Prop :=
   has_kind F (NumT (FloatT F32T)) (VALTYPE (PrimR F32R) Heapable Unr)
 | KF64 F :
   has_kind F (NumT (FloatT F64T)) (VALTYPE (PrimR F64R) Heapable Unr)
-| KSumVal F τs rs h l :
-  Forall2 (fun τ r => has_kind F τ (VALTYPE r h l)) τs rs ->
-  has_kind F (SumT τs) (VALTYPE (SumR rs) h l)
-| KSumMem F τs szs :
-  Forall2 (fun τ sz => has_kind F τ (MEMTYPE (Sized sz))) τs szs ->
-  has_kind F (SumT τs) (MEMTYPE (Sized (SumS szs)))
-| KProdVal F τs rs h l :
-  Forall2 (fun τ r => has_kind F τ (VALTYPE r h l)) τs rs ->
-  has_kind F (ProdT τs) (VALTYPE (ProdR rs) h l)
-| KProdMemSized F τs szs :
-  Forall2 (fun τ sz => has_kind F τ (MEMTYPE (Sized sz))) τs szs ->
-  has_kind F (ProdT τs) (MEMTYPE (Sized (ProdS szs)))
-| KProdMemUnsized F τs τ0 szs :
-  Forall2 (fun τ sz => has_kind F τ (MEMTYPE (Sized sz))) τs szs ->
-  has_kind F τ0 (MEMTYPE Unsized) ->
-  has_kind F (ProdT τs) (MEMTYPE Unsized)
-| KArray F τ sz :
-  has_kind F τ (MEMTYPE (Sized sz)) ->
+| KSumVal F τs ρs η γ :
+  Forall2 (fun τ ρ => has_kind F τ (VALTYPE ρ η γ)) τs ρs ->
+  has_kind F (SumT τs) (VALTYPE (SumR ρs) η γ)
+| KSumMem F τs ζs :
+  Forall2 (fun τ ζ => has_kind F τ (MEMTYPE ζ)) τs ζs ->
+  has_kind F (SumT τs) (MEMTYPE Unsized)
+| KSumMemSized F τs σs :
+  Forall2 (fun τ σ => has_kind F τ (MEMTYPE (Sized σ))) τs σs ->
+  has_kind F (SumT τs) (MEMTYPE (Sized (SumS σs)))
+| KProdVal F τs ρs η γ :
+  Forall2 (fun τ ρ => has_kind F τ (VALTYPE ρ η γ)) τs ρs ->
+  has_kind F (ProdT τs) (VALTYPE (ProdR ρs) η γ)
+| KProdMem F τs τn σs ζ :
+  Forall2 (fun τ σ => has_kind F τ (MEMTYPE (Sized σ))) τs σs ->
+  has_kind F τn (MEMTYPE ζ) ->
+  has_kind F (ProdT (τs ++ [τn])) (MEMTYPE Unsized)
+| KProdMemSized F τs σs :
+  Forall2 (fun τ σ => has_kind F τ (MEMTYPE (Sized σ))) τs σs ->
+  has_kind F (ProdT τs) (MEMTYPE (Sized (ProdS σs)))
+| KArray F τ σ :
+  has_kind F τ (MEMTYPE (Sized σ)) ->
   has_kind F (ArrayT τ) (MEMTYPE Unsized)
 | KExLoc F τ κ :
   has_kind (set fc_location_vars S F) τ κ ->
@@ -139,9 +143,6 @@ Inductive has_kind : function_ctx -> type -> kind -> Prop :=
 | KExSize F τ κ :
   has_kind (set fc_size_vars S F) τ κ ->
   has_kind F (ExT QSize τ) κ
-| KExSizity F τ κ :
-  has_kind (set fc_sizity_vars S F) τ κ ->
-  has_kind F (ExT QSizity τ) κ
 | KExType F τ κ0 κ :
   has_kind (set fc_type_vars (cons κ0) F) τ κ ->
   has_kind F (ExT (QType κ0) τ) κ
@@ -153,38 +154,38 @@ Inductive has_kind : function_ctx -> type -> kind -> Prop :=
   has_kind F (PtrT ℓ) (VALTYPE (PrimR PtrR) Heapable Unr)
 | KCap F ℓ τ :
   has_kind F (CapT ℓ τ) (VALTYPE (ProdR []) Unheapable Lin)
-| KRef F ℓ ω τ sz :
-  has_kind F τ (MEMTYPE sz) ->
+| KRef F ℓ ω τ ζ :
+  has_kind F τ (MEMTYPE ζ) ->
   has_kind F (RefT ω ℓ τ) (VALTYPE (PrimR PtrR) Heapable Lin)
-| KRefGC F ℓ τ sz :
-  has_kind F τ (MEMTYPE sz) ->
+| KRefGC F ℓ τ ζ :
+  has_kind F τ (MEMTYPE ζ) ->
   has_kind F (RefT OwnGC ℓ τ) (VALTYPE (PrimR PtrR) Heapable Unr)
-| KCodeRef F χ :
-  has_kind F (CodeRefT χ) (VALTYPE (PrimR I32R) Heapable Unr)
-| KRep F r0 r τ h l :
-  has_kind F τ (VALTYPE r0 h l) ->
-  has_kind F (RepT r τ) (VALTYPE r h l)
-| KPad F sz0 sz τ :
-  has_kind F τ (MEMTYPE (Sized sz0)) ->
-  has_kind F (PadT sz τ) (MEMTYPE (Sized sz))
-| KSer F τ r l :
-  has_kind F τ (VALTYPE r Heapable l) ->
-  has_kind F (SerT τ) (MEMTYPE (Sized (RepS r))).
+| KCodeRef F ϕ :
+  has_kind F (CodeRefT ϕ) (VALTYPE (PrimR I32R) Heapable Unr)
+| KRep F ρ0 ρ τ η γ :
+  has_kind F τ (VALTYPE ρ0 η γ) ->
+  has_kind F (RepT ρ τ) (VALTYPE ρ η γ)
+| KPad F σ0 σ τ :
+  has_kind F τ (MEMTYPE (Sized σ0)) ->
+  has_kind F (PadT σ τ) (MEMTYPE (Sized σ))
+| KSer F τ ρ γ :
+  has_kind F τ (VALTYPE ρ Heapable γ) ->
+  has_kind F (SerT τ) (MEMTYPE (Sized (RepS ρ))).
 
 Inductive has_rep : function_ctx -> type -> representation -> Prop :=
-| RepVALTYPE (F : function_ctx) (τ : type) (r : representation) (l : linearity) (h : heapability) :
-  has_kind F τ (VALTYPE r h l) ->
-  has_rep F τ r.
+| RepVALTYPE (F : function_ctx) (τ : type) (ρ : representation) (η : heapability) (γ : linearity) :
+  has_kind F τ (VALTYPE ρ η γ) ->
+  has_rep F τ ρ.
 
 Inductive is_unrestricted : function_ctx -> type -> Prop :=
-| UnrVALTYPE (F : function_ctx) (τ : type) (r : representation) (h : heapability) :
-  has_kind F τ (VALTYPE r h Unr) ->
+| UnrVALTYPE (F : function_ctx) (τ : type) (ρ : representation) (η : heapability) :
+  has_kind F τ (VALTYPE ρ η Unr) ->
   is_unrestricted F τ.
 
 Inductive module_ctx_ok : module_ctx -> Prop :=
-| MC_OK (τgs : list global_type) :
-  Forall (fun '(GlobalT _ τ) => is_unrestricted fc_empty τ) τgs ->
-  module_ctx_ok {| mc_globals := τgs |}.
+| MC_OK (gs : list (mutability * type)) :
+  Forall (fun '(_, τ) => is_unrestricted fc_empty τ) gs ->
+  module_ctx_ok {| mc_globals := gs |}.
 
 (* TODO *)
 Inductive num_instr_has_type : num_instr -> arrow_type -> Prop :=.
@@ -199,11 +200,11 @@ Inductive instr_has_type {A : Type} :
 | TUnreachable M F L L' ann τs1 τs2 le :
   L' = update_locals le L ->
   instr_has_type M F L (IUnreachable ann) (ArrowT τs1 τs2) L
-| TNum M F L ann en τa :
-  num_instr_has_type en τa ->
-  instr_has_type M F L (INum ann en) τa L
-| TNumConst M F L ann τn n :
-  instr_has_type M F L (INumConst ann τn n) (ArrowT [] [NumT τn]) L
+| TNum M F L ann en χ :
+  num_instr_has_type en χ ->
+  instr_has_type M F L (INum ann en) χ L
+| TNumConst M F L ann ν n :
+  instr_has_type M F L (INumConst ann ν n) (ArrowT [] [NumT ν]) L
 | TBlock M F F' L L' ann τs1 τs2 le es :
   F' = set fc_labels (cons (τs2, L')) F ->
   L' = update_locals le L ->
@@ -213,11 +214,11 @@ Inductive instr_has_type {A : Type} :
   F' = set fc_labels (cons (τs1, L)) F ->
   expr_has_type M F L es (ArrowT τs1 τs2) L ->
   instr_has_type M F L (ILoop ann (ArrowT τs1 τs2) es) (ArrowT τs1 τs2) L
-| TIte M F L L' ann τa le es1 es2 :
+| TIte M F L L' ann χ le es1 es2 :
   L' = update_locals le L ->
-  expr_has_type M F L es1 τa L' ->
-  expr_has_type M F L es2 τa L' ->
-  instr_has_type M F L (IIte ann τa le es1 es2) τa L'
+  expr_has_type M F L es1 χ L' ->
+  expr_has_type M F L es2 χ L' ->
+  instr_has_type M F L (IIte ann χ le es1 es2) χ L'
 | TBr M F L L' ann n τs τs1 τs2 le :
   L' = update_locals le L ->
   F.(fc_labels) !! n = Some (τs, L) ->
@@ -235,27 +236,27 @@ Inductive instr_has_type {A : Type} :
   L' = update_locals le L ->
   Forall (is_unrestricted F) τs1 ->
   instr_has_type M F L (IReturn ann) (ArrowT (τs1 ++ τs) τs2) L'
-| TLocalGet M F L L' ann n τ r :
+| TLocalGet M F L L' ann n τ ρ :
   L !! n = Some τ ->
-  has_rep F τ r ->
-  L' = <[ n := RepT r (ProdT []) ]> L ->
+  has_rep F τ ρ ->
+  L' = <[ n := RepT ρ (ProdT []) ]> L ->
   instr_has_type M F L (ILocalGet ann n) (ArrowT [] [τ]) L'
 | TLocalGetUnr M F L ann n τ :
   L !! n = Some τ ->
   is_unrestricted F τ ->
   instr_has_type M F L (ILocalGet ann n) (ArrowT [] [τ]) L
-| TLocalSet M F L L' ann n τ τ' r :
+| TLocalSet M F L L' ann n τ τ' ρ :
   L' = <[ n := τ' ]> L ->
   L !! n = Some τ ->
   is_unrestricted F τ ->
-  has_rep F τ r ->
-  has_rep F τ' r ->
+  has_rep F τ ρ ->
+  has_rep F τ' ρ ->
   instr_has_type M F L (ILocalSet ann n) (ArrowT [τ'] []) L'
 | TGlobalGet M F L ann n m τ :
-  M.(mc_globals) !! n = Some (GlobalT m τ) ->
+  M.(mc_globals) !! n = Some (m, τ) ->
   instr_has_type M F L (IGlobalGet ann n) (ArrowT [] [τ]) L
 | TGlobalSet M F L ann n m τ :
-  M.(mc_globals) !! n = Some (GlobalT m τ) ->
+  M.(mc_globals) !! n = Some (m, τ) ->
   instr_has_type M F L (IGlobalSet ann n) (ArrowT [τ] []) L
 
 with expr_has_type {A : Type} :
